Groundwork for delegation refinement.

src/Common/Ensembles/IndexedEnsembles.v
@@ -2,7 +2,10 @@ Require Import Coq.Lists.List
         Coq.Strings.String
         Coq.Logic.FunctionalExtensionality
         Coq.Sorting.Permutation Coq.Sets.Ensembles
-        Fiat.Common.List.PermutationFacts.
+        Fiat.Common.DecideableEnsembles
+        Fiat.Common.List.PermutationFacts
+        Fiat.Common.List.ListMorphisms
+        Fiat.Common.List.ListFacts.
 
 Class UnConstrRelationAbsRClass {A B : Type} :=
   { UnConstrRelationAbsR : Ensemble A -> B -> Prop }.
@@ -25,7 +28,7 @@ Section IndexedEnsembles.
   Definition IndexedEnsembleSubtract
              (element : ElementType)
              (ens : IndexedEnsemble)
-  : IndexedEnsemble :=
+    : IndexedEnsemble :=
     fun element' => indexedElement element' <> element /\ ens element'.
 
   (* 'Deleting' a set of tuples [R] from a relation [F] is the same
@@ -39,7 +42,7 @@ Section IndexedEnsembles.
              (ens : IndexedEnsemble)
              (cond : Ensemble ElementType)
              (updateR : relation ElementType)
-  : IndexedEnsemble
+    : IndexedEnsemble
     := fun e => (exists f: IndexedElement, ((ens f) /\ cond (indexedElement f) /\ updateR (indexedElement f) (indexedElement e))
                                            /\ elementIndex e = elementIndex f) \/
                 ((ens e) /\ Complement _ (fun f => cond (indexedElement f)) e).
@@ -54,9 +57,9 @@ Section IndexedEnsembles.
   Definition UnConstrFreshIdx
              (ensemble : IndexedEnsemble)
              (bound : nat) :=
-  forall element,
-    ensemble element
-    -> lt (elementIndex element) bound.
+    forall element,
+      ensemble element
+      -> lt (elementIndex element) bound.
 
   Definition EnsembleIndexedListEquivalence
              (ensemble : IndexedEnsemble)
@@ -71,20 +74,20 @@ Section IndexedEnsembles.
 
   Ltac destruct_EnsembleIndexedListEquivalence :=
     match goal with
-        H : EnsembleIndexedListEquivalence ?or ?nr |- _ =>
-        let bnd := fresh "bnd" in
-        let fresh_bnd := fresh "fresh_bnd" in
-        let lor := fresh "l" or in
-        let eqv_or := fresh "eqv_" or in
-        let NoDup_lor := fresh "NoDup_" or in
-        let eqv_r_n := fresh "eqv_nr" in
-        let H' := fresh in
-        pose proof H as H';
+      H : EnsembleIndexedListEquivalence ?or ?nr |- _ =>
+      let bnd := fresh "bnd" in
+      let fresh_bnd := fresh "fresh_bnd" in
+      let lor := fresh "l" or in
+      let eqv_or := fresh "eqv_" or in
+      let NoDup_lor := fresh "NoDup_" or in
+      let eqv_r_n := fresh "eqv_nr" in
+      let H' := fresh in
+      pose proof H as H';
         destruct H' as [[bnd fresh_bnd] [lor [eqv_or [eqv_r_n NoDup_lor]]]]
     end.
 
   Lemma Permutation_EnsembleIndexedListEquivalence
-  : forall ensemble (l l' : list _),
+    : forall ensemble (l l' : list _),
       EnsembleIndexedListEquivalence ensemble l
       -> Permutation l l'
       -> EnsembleIndexedListEquivalence ensemble l'.
@@ -111,18 +114,97 @@ Section IndexedEnsembles.
     induction l1; simpl; constructor; inversion H; subst; eauto using in_map.
   Qed.
 
+  Definition IndexedEnsemble_Intersection
+             (ens : IndexedEnsemble)
+             (ens' : Ensemble ElementType)
+    : IndexedEnsemble :=
+    fun element' => ens element' /\ ens' (indexedElement element').
+
+  Definition FiniteEnsemble (P : IndexedEnsemble)
+    := exists l, UnIndexedEnsembleListEquivalence P l.
+
+  Lemma NoDup_filter_map :
+    forall (f : _ -> bool)
+           (l : list _),
+      NoDup (map elementIndex l)
+      -> NoDup
+           (map elementIndex
+                (filter (fun a => f (indexedElement a)) l)) .
+  Proof.
+    induction l; simpl.
+    - constructor.
+    - case_eq (f (indexedElement a)); simpl; intros; inversion H0; subst; eauto.
+      constructor; eauto.
+      unfold not; intros; apply H3.
+      revert H1; clear; induction l; simpl.
+      + eauto.
+      + case_eq (f (indexedElement a0)); simpl; intros; intuition.
+  Qed.
+
+
+  Lemma UnIndexedEnsembleListEquivalence_filter
+    : forall R P (P_dec : DecideableEnsemble (A := ElementType) P) l,
+      UnIndexedEnsembleListEquivalence R l
+      -> UnIndexedEnsembleListEquivalence (IndexedEnsemble_Intersection R P)
+                                          (filter (@DecideableEnsembles.dec _ P P_dec) l).
+  Proof.
+    destruct 1.
+    eexists (filter (fun x => DecideableEnsembles.dec (indexedElement x)) x); simpl; intuition.
+    - rewrite <- filter_map, H0; reflexivity.
+    - inversion H1.
+      rewrite H in H3.
+      revert H3 H4; clear; induction x; simpl; intuition subst.
+      + apply dec_decides_P in H4; rewrite H4; simpl; intuition.
+      + find_if_inside; simpl; eauto.
+    - apply filter_In in H1; intuition.
+      apply dec_decides_P in H4; econstructor; eauto.
+      apply H; eauto.
+    - eauto using NoDup_filter_map.
+  Qed.
+
+  Lemma Permutation_UnIndexedEnsembleListEquivalence
+    : forall ensemble (l l' : list ElementType),
+      UnIndexedEnsembleListEquivalence ensemble l
+      -> Permutation l l'
+      -> UnIndexedEnsembleListEquivalence ensemble l'.
+  Proof.
+    simpl; intros.
+    destruct H; intuition; symmetry in H0.
+    destruct (PermutationFacts.permutation_map_base _ H0 _ H1)
+      as [l'' [l''_eq H']].
+    econstructor; split; intuition eauto.
+    rewrite H'; eapply H; eauto.
+    rewrite H' in H2; eapply H; eauto.
+    eapply PermutationFacts.NoDup_modulo_permutation.
+    eexists (map elementIndex x).
+    intuition. apply Permutation_map. auto.
+  Qed.
+
+  Lemma Permutation_UnIndexedEnsembleListEquivalence'
+    : forall ensemble (l l' : list _),
+      UnIndexedEnsembleListEquivalence ensemble l
+      -> UnIndexedEnsembleListEquivalence ensemble l'
+      -> Permutation l l'.
+  Proof.
+    simpl; intros.
+    destruct H; destruct H0; intuition subst.
+    setoid_rewrite H0 in H2.
+    eapply Permutation_map.
+    eapply NoDup_Permutation; eauto using NoDup_IndexedElement.
+  Qed.
+
 End IndexedEnsembles.
 
 Ltac destruct_EnsembleIndexedListEquivalence :=
   match goal with
-      H : EnsembleIndexedListEquivalence ?or ?nr |- _ =>
-      let bnd := fresh "bnd" in
-      let fresh_bnd := fresh "fresh_bnd" in
-      let lor := fresh "l" or in
-      let eqv_or := fresh "eqv_" or in
-      let NoDup_lor := fresh "NoDup_" or in
-      let eqv_r_n := fresh "eqv_nr" in
-      let H' := fresh in
-      pose proof H as H';
-        destruct H' as [[bnd fresh_bnd] [lor [eqv_or [eqv_r_n NoDup_lor]]]]
+    H : EnsembleIndexedListEquivalence ?or ?nr |- _ =>
+    let bnd := fresh "bnd" in
+    let fresh_bnd := fresh "fresh_bnd" in
+    let lor := fresh "l" or in
+    let eqv_or := fresh "eqv_" or in
+    let NoDup_lor := fresh "NoDup_" or in
+    let eqv_r_n := fresh "eqv_nr" in
+    let H' := fresh in
+    pose proof H as H';
+      destruct H' as [[bnd fresh_bnd] [lor [eqv_or [eqv_r_n NoDup_lor]]]]
   end.
