src/QueryStructure/Implementation/Operations/General/QueryRefinements.v
@@ -28,9 +28,9 @@ Import Coq.Vectors.VectorDef.VectorNotations.
 Local Transparent Query_For Count Max MaxN MaxZ Sum SumN SumZ.
 
 Lemma refine_Count {A} rows
-: refine (@Count A rows)
-         (l <- rows;
-          ret (List.length l)).
+  : refine (@Count A rows)
+           (l <- rows;
+            ret (List.length l)).
 Proof. reflexivity. Qed.
 
 Lemma refine_FoldAggregateOption {A} (rows: Comp (list A)) (updater: A -> A -> A) :
@@ -82,7 +82,7 @@ Lemma refine_MaxZ rows :
 Proof. reflexivity. Qed.
 
 Lemma refine_For
-: forall ResultT (bod : Comp (list ResultT)),
+  : forall ResultT (bod : Comp (list ResultT)),
     refine (For bod)%QuerySpec
            (result <- bod;
             {l | Permutation result l}).
@@ -106,7 +106,7 @@ Tactic Notation "t_morphism" reference(symb) :=
   intros * H; unfold symb; rewrite H; reflexivity.
 
 Add Parametric Morphism ResultT
-: (@Query_For ResultT)
+  : (@Query_For ResultT)
     with signature (refine ==> refine)
       as refine_refine_For.
 Proof.
@@ -114,7 +114,7 @@ Proof.
 Qed.
 
 Add Parametric Morphism ResultT
-: (@Count ResultT)
+  : (@Count ResultT)
     with signature (refine ==> refine)
       as refine_refine_Count.
 Proof.
@@ -180,7 +180,7 @@ Proof.
 Qed.
 
 Lemma refine_Count_bind_bind_app {A}
-: forall (l l' : Comp (list A)),
+  : forall (l l' : Comp (list A)),
     refine (Count (la <- l;
                    la' <- l';
                    {l | Permutation.Permutation (la ++ la') l}))
@@ -203,7 +203,7 @@ Definition UnConstrQuery_In {ResultT}
     QueryResultComp (GetUnConstrRelation qs R) bod.
 
 Lemma refine_flatten_CompList_func {A B}
-: forall (l : list A) (f f' : A -> Comp (list B)),
+  : forall (l : list A) (f f' : A -> Comp (list B)),
     pointwise_relation _ refine f f'
     -> refine (flatten_CompList (map f l))
               (flatten_CompList (map f' l)).
@@ -215,7 +215,7 @@ Proof.
 Qed.
 
 Add Parametric Morphism {ResultT} P
-: (@Query_Where ResultT P)
+  : (@Query_Where ResultT P)
     with signature (refine ==> refine)
       as refine_Query_Where_In.
 Proof.
@@ -224,7 +224,7 @@ Proof.
 Qed.
 
 Add Parametric Morphism {ResultT} qsSchema qs R
-: (@UnConstrQuery_In ResultT qsSchema qs R)
+  : (@UnConstrQuery_In ResultT qsSchema qs R)
     with signature (pointwise_relation _ refine ==> refine)
       as refine_UnConstrQuery_In.
 Proof.
@@ -244,13 +244,13 @@ Definition Join_Comp_Lists
            {a : A}
            (l' : list (ilist2 (B := f) As))
            (c : ilist2 (B := f) As -> Comp (list (f a)))
-: Comp (list (ilist2 (B := f) (Vector.cons _ a _ As))) :=
+  : Comp (list (ilist2 (B := f) (Vector.cons _ a _ As))) :=
   flatten_CompList (map (fun l' => l <- c l'; ret (map (fun fa => icons2 fa l') l)) l').
 
 Definition Build_single_Tuple_list
            {heading}
            (l : list (@RawTuple heading))
-: list (ilist2 (B := @RawTuple) (Vector.cons _ heading _ (Vector.nil _)))
+  : list (ilist2 (B := @RawTuple) (Vector.cons _ heading _ (Vector.nil _)))
   := map (fun a => icons2 a (inil2)) l.
 
 Lemma filter_and_join_ilist_tail
@@ -259,7 +259,7 @@ Lemma filter_and_join_ilist_tail
       {a}
       {As : Vector.t A n}
       (f' : A -> Type)
-: forall
+  : forall
     (f : (ilist2 (B := f') As) -> bool)
     (s1 : list (ilist2 (B := f') As))
     (s2 : ilist2 (B := f') As -> Comp (list (f' a)))
@@ -289,7 +289,7 @@ Proof.
   - intros v Comp_v;  computes_to_inv; subst.
     pose proof (IHs1 (fun a In_a => H _ (or_intror In_a)) _
                      (BindComputes _ (fun x => ret (_ x)) _ _ Comp_v'0 (ReturnComputes _))).
-     computes_to_inv.
+    computes_to_inv.
     case_eq (f a0); intros a0_eq; simpl.
     + repeat (computes_to_econstructor; eauto).
       rewrite !filter_app, !filter_map, H0', filter_and; simpl.
@@ -312,7 +312,7 @@ Corollary filter_join_ilist2_tail
           {a}
           {As : Vector.t A n}
           (f' : A -> Type)
-: forall
+  : forall
     (f : (ilist2 (B := f') As) -> bool)
     (s1 : list (ilist2 (B := f') As))
     (s2 : ilist2 (B := f') As -> Comp (list (f' a))),
@@ -328,16 +328,16 @@ Qed.
 
 
 Lemma refine_Join_Comp_Lists_filter_tail
-: forall {n} heading headings
-         (f : ilist2 (n := n) (B := @RawTuple) headings -> bool)
-         (filter_rest : ilist2 (B := @RawTuple) (heading :: headings) -> bool)
-         (ResultT : Type)
-         (resultComp : _ -> Comp (list ResultT))
-         (l2 : ilist2 (B:= @RawTuple) headings
-               -> Comp (list (@RawTuple heading))),
+  : forall {n} heading headings
+           (f : ilist2 (n := n) (B := @RawTuple) headings -> bool)
+           (filter_rest : ilist2 (B := @RawTuple) (heading :: headings) -> bool)
+           (ResultT : Type)
+           (resultComp : _ -> Comp (list ResultT))
+           (l2 : ilist2 (B:= @RawTuple) headings
+                 -> Comp (list (@RawTuple heading))),
     (forall a : ilist2 (B := @RawTuple) headings,
-     exists v : list (@RawTuple heading),
-       refine (l2 a) (ret v))
+        exists v : list (@RawTuple heading),
+          refine (l2 a) (ret v))
     ->
     forall l1,
       refine
@@ -368,7 +368,7 @@ Proof.
       rewrite filter_and, a_eq, filter_true.
       eapply FlattenCompList.flatten_CompList_app; eauto.
     + destruct (H a); eauto.
-       computes_to_inv; subst; computes_to_econstructor; eauto.
+      computes_to_inv; subst; computes_to_econstructor; eauto.
       pose (IHl1 l2 H _ (BindComputes _ _ _ _ Comp_v Comp_v'));  computes_to_inv; subst.
       computes_to_econstructor; eauto.
       unfold List_Query_In.
@@ -380,17 +380,17 @@ Qed.
 (* A version of [refine_Join_Comp_Lists_filter_tail] for the case that
       the realizeablity of [l2] depends on the elements of [l1]*)
 Lemma refine_Join_Comp_Lists_filter_tail_cond
-: forall n heading headings
-         (f : ilist2 (n := n) (B := @RawTuple) (headings) -> bool)
-         (filter_rest : ilist2 (B := @RawTuple) (heading :: headings) -> bool)
-         (ResultT : Type)
-         (resultComp : _ -> Comp (list ResultT))
-         (l1 : list (ilist2 (B := @RawTuple) headings))
-         (l2 : ilist2 (B := @RawTuple) headings
-               -> Comp (list (@RawTuple heading))),
+  : forall n heading headings
+           (f : ilist2 (n := n) (B := @RawTuple) (headings) -> bool)
+           (filter_rest : ilist2 (B := @RawTuple) (heading :: headings) -> bool)
+           (ResultT : Type)
+           (resultComp : _ -> Comp (list ResultT))
+           (l1 : list (ilist2 (B := @RawTuple) headings))
+           (l2 : ilist2 (B := @RawTuple) headings
+                 -> Comp (list (@RawTuple heading))),
     (forall a : ilist2 (B := @RawTuple) headings,
-       List.In a l1 -> exists v : list (@RawTuple heading),
-                         refine (l2 a) (ret v))
+        List.In a l1 -> exists v : list (@RawTuple heading),
+          refine (l2 a) (ret v))
     -> refine
          (l' <- Join_Comp_Lists l1 l2;
           List_Query_In
@@ -418,7 +418,7 @@ Proof.
       rewrite filter_and, a_eq, filter_true.
       eapply FlattenCompList.flatten_CompList_app; eauto.
     + destruct (H a); eauto.
-       computes_to_inv; subst; computes_to_econstructor; eauto.
+      computes_to_inv; subst; computes_to_econstructor; eauto.
       pose (IHl1 l2 (fun a In_a => H _ (or_intror In_a)) _ (BindComputes _ _ _ _ Comp_v Comp_v'));  computes_to_inv; subst.
       computes_to_econstructor; eauto.
       unfold List_Query_In.
@@ -436,7 +436,7 @@ Definition Join_Filtered_Comp_Lists
            (l' : list (ilist2 (B := f) As))
            (c : ilist2 (B := f) As -> Comp (list (f a)))
            (cond : ilist2 (B := f) (a :: As) -> bool)
-: Comp (list (ilist2 (B := f) (a :: As))) :=
+  : Comp (list (ilist2 (B := f) (a :: As))) :=
   l <- Join_Comp_Lists l' c;
   ret (filter cond l).
 
@@ -446,28 +446,28 @@ Lemma Join_Filtered_Comp_Lists_id
       {f : A -> Type}
       {As : Vector.t A n}
       {a : A}
-: forall (l' : list (ilist2 (B := f) As))
-         (c : ilist2 (B := f) As -> Comp (list (f a))),
+  : forall (l' : list (ilist2 (B := f) As))
+           (c : ilist2 (B := f) As -> Comp (list (f a))),
     refine (Join_Comp_Lists l' c)
            (Join_Filtered_Comp_Lists l' c (fun _ => true)).
-  unfold Join_Filtered_Comp_Lists; setoid_rewrite filter_true.
-  intros; rewrite refineEquiv_unit_bind; reflexivity.
+      unfold Join_Filtered_Comp_Lists; setoid_rewrite filter_true.
+      intros; rewrite refineEquiv_unit_bind; reflexivity.
 Qed.
 
 Lemma refine_Join_Filtered_Comp_Lists_filter_tail_andb
-: forall n heading headings
-         (f g : ilist2 (n := S n) (B := @RawTuple) (heading :: headings) -> bool)
-         (ResultT : Type)
-         (resultComp : ilist2 (B := @RawTuple) (heading :: headings) ->
-                       Comp (list ResultT))
-         (l2 : ilist2 (B := @RawTuple) headings -> Comp (list RawTuple))
-         (cond : ilist2 (B := @RawTuple) (heading :: headings) -> bool),
-  forall l1 : list (ilist2 (B := @RawTuple) headings),
-    refine
-      (l' <- Join_Filtered_Comp_Lists l1 l2 cond;
-       List_Query_In (filter (fun a => f a && g a) l') resultComp)
-      (l' <- Join_Filtered_Comp_Lists l1 l2 (fun a => cond a && f a);
-       List_Query_In (filter g l') resultComp).
+  : forall n heading headings
+           (f g : ilist2 (n := S n) (B := @RawTuple) (heading :: headings) -> bool)
+           (ResultT : Type)
+           (resultComp : ilist2 (B := @RawTuple) (heading :: headings) ->
+                         Comp (list ResultT))
+           (l2 : ilist2 (B := @RawTuple) headings -> Comp (list RawTuple))
+           (cond : ilist2 (B := @RawTuple) (heading :: headings) -> bool),
+    forall l1 : list (ilist2 (B := @RawTuple) headings),
+      refine
+        (l' <- Join_Filtered_Comp_Lists l1 l2 cond;
+         List_Query_In (filter (fun a => f a && g a) l') resultComp)
+        (l' <- Join_Filtered_Comp_Lists l1 l2 (fun a => cond a && f a);
+         List_Query_In (filter g l') resultComp).
 Proof.
   intros; revert l2.
   unfold Join_Filtered_Comp_Lists, Join_Comp_Lists; induction l1; simpl;
@@ -480,19 +480,19 @@ Proof.
 Qed.
 
 Corollary refine_Join_Filtered_Comp_Lists_filter_tail
-: forall n heading headings
-         (f : ilist2 (n := S n) (B := @RawTuple) (heading :: headings) -> bool)
-         (ResultT : Type)
-         (resultComp : ilist2 (B := @RawTuple) (heading :: headings) ->
-                       Comp (list ResultT))
-         (l2 : ilist2 (B := @RawTuple) headings -> Comp (list RawTuple))
-         (cond : ilist2 (B := @RawTuple) (heading :: headings) -> bool),
-  forall l1 : list (ilist2 (B := @RawTuple) headings),
-    refine
-      (l' <- Join_Filtered_Comp_Lists l1 l2 cond;
-       List_Query_In (filter f l') resultComp)
-      (l' <- Join_Filtered_Comp_Lists l1 l2 (fun a => cond a && f a);
-       List_Query_In l' resultComp).
+  : forall n heading headings
+           (f : ilist2 (n := S n) (B := @RawTuple) (heading :: headings) -> bool)
+           (ResultT : Type)
+           (resultComp : ilist2 (B := @RawTuple) (heading :: headings) ->
+                         Comp (list ResultT))
+           (l2 : ilist2 (B := @RawTuple) headings -> Comp (list RawTuple))
+           (cond : ilist2 (B := @RawTuple) (heading :: headings) -> bool),
+    forall l1 : list (ilist2 (B := @RawTuple) headings),
+      refine
+        (l' <- Join_Filtered_Comp_Lists l1 l2 cond;
+         List_Query_In (filter f l') resultComp)
+        (l' <- Join_Filtered_Comp_Lists l1 l2 (fun a => cond a && f a);
+         List_Query_In l' resultComp).
 Proof.
   intros;
   pose proof (@refine_Join_Filtered_Comp_Lists_filter_tail_andb
@@ -500,22 +500,22 @@ Proof.
   setoid_rewrite filter_true in r.
   intros v Comp_v.
   apply r in Comp_v.
-   computes_to_inv; subst.
+  computes_to_inv; subst.
   rewrite filter_and, filter_true in Comp_v'.
   eauto.
 Qed.
 
 Lemma refine_Join_Filtered_Comp_Lists_filter_hd_andb
-: forall n heading headings
-         (f : ilist2 (n := n) (B := @RawTuple) headings -> bool)
-         (g : ilist2 (B := @RawTuple) (heading :: headings) -> bool)
-         (ResultT : Type)
-         (resultComp : ilist2 (B := @RawTuple) (heading :: headings) ->
-                       Comp (list ResultT))
-         (l2 : ilist2 (B := @RawTuple) headings -> Comp (list RawTuple))
-         (cond : ilist2 (B := @RawTuple) (heading :: headings) -> bool),
+  : forall n heading headings
+           (f : ilist2 (n := n) (B := @RawTuple) headings -> bool)
+           (g : ilist2 (B := @RawTuple) (heading :: headings) -> bool)
+           (ResultT : Type)
+           (resultComp : ilist2 (B := @RawTuple) (heading :: headings) ->
+                         Comp (list ResultT))
+           (l2 : ilist2 (B := @RawTuple) headings -> Comp (list RawTuple))
+           (cond : ilist2 (B := @RawTuple) (heading :: headings) -> bool),
     (forall a : ilist2 (B := @RawTuple) headings,
-     exists v : list RawTuple, refine (l2 a) (ret v)) ->
+        exists v : list RawTuple, refine (l2 a) (ret v)) ->
     forall l1 : list (ilist2 (B := @RawTuple) headings),
       refine
         (l' <- Join_Filtered_Comp_Lists l1 l2 cond;
@@ -532,31 +532,31 @@ Proof.
   - repeat setoid_rewrite refineEquiv_bind_unit; simpl; reflexivity.
   - case_eq (f a); simpl; intros a_eq v Comp_v.
     +  computes_to_inv; subst; computes_to_econstructor; eauto.
-      unfold List_Query_In in Comp_v'.
-      rewrite !filter_app, !filter_map, !map_app, !map_map in Comp_v'.
-      apply FlattenCompList.flatten_CompList_app_inv' in Comp_v'.
-      destruct_ex; split_and.
-      assert (computes_to (l' <- l <- FlattenCompList.flatten_CompList
-                              (map
-                                 (fun l' : ilist2 (B := @RawTuple) headings =>
-                                    l <- l2 l';
-                                  ret (map (fun fa : RawTuple => icons2 fa l') l))
-                                 (filter f l1));
-                           ret (filter cond l);
-                           List_Query_In (filter g l') resultComp) x0)
-        as H'
-          by (setoid_rewrite <- filter_and in H3;
-              repeat econstructor; eauto;
-              setoid_rewrite <- filter_and; eauto).
-      pose (IHl1 l2 H _ H');  computes_to_inv; subst.
-      computes_to_econstructor; eauto.
-      unfold List_Query_In.
-      repeat rewrite filter_app, filter_map.
-      repeat rewrite map_app, map_map; simpl.
-      rewrite filter_and, a_eq, filter_true.
-      eapply FlattenCompList.flatten_CompList_app; eauto.
+       unfold List_Query_In in Comp_v'.
+       rewrite !filter_app, !filter_map, !map_app, !map_map in Comp_v'.
+       apply FlattenCompList.flatten_CompList_app_inv' in Comp_v'.
+       destruct_ex; split_and.
+       assert (computes_to (l' <- l <- FlattenCompList.flatten_CompList
+                               (map
+                                  (fun l' : ilist2 (B := @RawTuple) headings =>
+                                     l <- l2 l';
+                                   ret (map (fun fa : RawTuple => icons2 fa l') l))
+                                  (filter f l1));
+                            ret (filter cond l);
+                            List_Query_In (filter g l') resultComp) x0)
+         as H'
+           by (setoid_rewrite <- filter_and in H3;
+               repeat econstructor; eauto;
+               setoid_rewrite <- filter_and; eauto).
+       pose (IHl1 l2 H _ H');  computes_to_inv; subst.
+       computes_to_econstructor; eauto.
+       unfold List_Query_In.
+       repeat rewrite filter_app, filter_map.
+       repeat rewrite map_app, map_map; simpl.
+       rewrite filter_and, a_eq, filter_true.
+       eapply FlattenCompList.flatten_CompList_app; eauto.
     + destruct (H a); eauto.
-       computes_to_inv; subst; computes_to_econstructor; eauto.
+      computes_to_inv; subst; computes_to_econstructor; eauto.
       assert (computes_to (l' <- l <- FlattenCompList.flatten_CompList
                               (map
                                  (fun l' : ilist2 (B := @RawTuple) headings =>
@@ -575,15 +575,15 @@ Proof.
 Qed.
 
 Lemma refine_Join_Filtered_Comp_Lists_filter_hd
-: forall n heading headings
-         (f : ilist2 (n := n) (B := @RawTuple) headings -> bool)
-         (ResultT : Type)
-         (resultComp : ilist2 (B := @RawTuple) (heading :: headings) ->
-                       Comp (list ResultT))
-         (l2 : ilist2 (B := @RawTuple) headings -> Comp (list RawTuple))
-         (cond : ilist2 (B := @RawTuple) (heading :: headings) -> bool),
+  : forall n heading headings
+           (f : ilist2 (n := n) (B := @RawTuple) headings -> bool)
+           (ResultT : Type)
+           (resultComp : ilist2 (B := @RawTuple) (heading :: headings) ->
+                         Comp (list ResultT))
+           (l2 : ilist2 (B := @RawTuple) headings -> Comp (list RawTuple))
+           (cond : ilist2 (B := @RawTuple) (heading :: headings) -> bool),
     (forall a : ilist2 (B := @RawTuple) headings,
-     exists v : list RawTuple, refine (l2 a) (ret v)) ->
+        exists v : list RawTuple, refine (l2 a) (ret v)) ->
     forall l1 : list (ilist2 (B := @RawTuple) headings),
       refine
         (l' <- Join_Filtered_Comp_Lists l1 l2 cond;
@@ -599,7 +599,7 @@ Proof.
   setoid_rewrite filter_true in r.
   intros v Comp_v.
   apply r in Comp_v.
-   computes_to_inv; subst.
+  computes_to_inv; subst.
   rewrite filter_and, filter_true in Comp_v'.
   eauto.
 Qed.
@@ -610,9 +610,9 @@ Lemma Join_Filtered_Comp_Lists_ExtensionalEq_filters
       {f : A -> Type}
       {As : Vector.t A n}
       {a : A}
-: forall (l' : list (ilist2 (B := f) As))
-         (c : ilist2 (B := f) As -> Comp (list (f a)))
-         (g g' : ilist2 (B := f) (a :: As) -> bool),
+  : forall (l' : list (ilist2 (B := f) As))
+           (c : ilist2 (B := f) As -> Comp (list (f a)))
+           (g g' : ilist2 (B := f) (a :: As) -> bool),
     ExtensionalEq g g'
     -> refine (Join_Filtered_Comp_Lists l' c g)
               (Join_Filtered_Comp_Lists l' c g').
@@ -624,18 +624,18 @@ Qed.
 
 
 Lemma refine_Join_Join_Filtered_Comp_Lists_filter_tail_andb
-: forall n heading1 heading2 headings
-         (f g : ilist2 (n := S n) (B := @RawTuple) (heading1 :: headings) -> bool)
-         (l2 : ilist2 (B := @RawTuple) headings -> Comp (list RawTuple))
-         (l2' : ilist2 (B := @RawTuple) (heading1 :: headings) -> Comp (list RawTuple))
-         (cond1 : ilist2 (B := @RawTuple) (heading1 :: headings) -> bool)
-         (cond2 : ilist2 (B := @RawTuple) (heading2 :: heading1 :: headings) -> bool),
-  forall l1 : list (ilist2 (B := @RawTuple) headings),
-    refine
-      (l <- Join_Filtered_Comp_Lists l1 l2 cond1;
-       Join_Filtered_Comp_Lists (filter (fun a => f a && g a) l) l2' cond2)
-      (l <- Join_Filtered_Comp_Lists l1 l2 (fun a => cond1 a && f a);
-       Join_Filtered_Comp_Lists (filter g l) l2' cond2).
+  : forall n heading1 heading2 headings
+           (f g : ilist2 (n := S n) (B := @RawTuple) (heading1 :: headings) -> bool)
+           (l2 : ilist2 (B := @RawTuple) headings -> Comp (list RawTuple))
+           (l2' : ilist2 (B := @RawTuple) (heading1 :: headings) -> Comp (list RawTuple))
+           (cond1 : ilist2 (B := @RawTuple) (heading1 :: headings) -> bool)
+           (cond2 : ilist2 (B := @RawTuple) (heading2 :: heading1 :: headings) -> bool),
+    forall l1 : list (ilist2 (B := @RawTuple) headings),
+      refine
+        (l <- Join_Filtered_Comp_Lists l1 l2 cond1;
+         Join_Filtered_Comp_Lists (filter (fun a => f a && g a) l) l2' cond2)
+        (l <- Join_Filtered_Comp_Lists l1 l2 (fun a => cond1 a && f a);
+         Join_Filtered_Comp_Lists (filter g l) l2' cond2).
 Proof.
   intros; revert l2 l2'.
   unfold Join_Filtered_Comp_Lists, Join_Comp_Lists; induction l1; simpl;
@@ -650,18 +650,18 @@ Proof.
 Qed.
 
 Corollary refine_Join_Join_Filtered_Comp_Lists_filter_tail
-: forall n heading1 heading2 headings
-         (f : ilist2 (n := S n) (B := @RawTuple) (heading1 :: headings) -> bool)
-         (l2 : ilist2 (B := @RawTuple) headings -> Comp (list RawTuple))
-         (l2' : ilist2 (B := @RawTuple) (heading1 :: headings) -> Comp (list RawTuple))
-         (cond1 : ilist2 (B := @RawTuple) (heading1 :: headings) -> bool)
-         (cond2 : ilist2 (B := @RawTuple) (heading2 :: heading1 :: headings) -> bool),
-  forall l1 : list (ilist2 (B := @RawTuple) headings),
-    refine
-      (l <- Join_Filtered_Comp_Lists l1 l2 cond1;
-       Join_Filtered_Comp_Lists (filter f l) l2' cond2)
-      (l <- Join_Filtered_Comp_Lists l1 l2 (fun a => cond1 a && f a);
-       Join_Filtered_Comp_Lists l l2' cond2).
+  : forall n heading1 heading2 headings
+           (f : ilist2 (n := S n) (B := @RawTuple) (heading1 :: headings) -> bool)
+           (l2 : ilist2 (B := @RawTuple) headings -> Comp (list RawTuple))
+           (l2' : ilist2 (B := @RawTuple) (heading1 :: headings) -> Comp (list RawTuple))
+           (cond1 : ilist2 (B := @RawTuple) (heading1 :: headings) -> bool)
+           (cond2 : ilist2 (B := @RawTuple) (heading2 :: heading1 :: headings) -> bool),
+    forall l1 : list (ilist2 (B := @RawTuple) headings),
+      refine
+        (l <- Join_Filtered_Comp_Lists l1 l2 cond1;
+         Join_Filtered_Comp_Lists (filter f l) l2' cond2)
+        (l <- Join_Filtered_Comp_Lists l1 l2 (fun a => cond1 a && f a);
+         Join_Filtered_Comp_Lists l l2' cond2).
 Proof.
   intros;
   pose proof (@refine_Join_Join_Filtered_Comp_Lists_filter_tail_andb
@@ -669,21 +669,21 @@ Proof.
   setoid_rewrite filter_true in r.
   intros v Comp_v.
   apply r in Comp_v.
-   computes_to_inv; subst.
+  computes_to_inv; subst.
   rewrite filter_and, filter_true in Comp_v'.
   eauto.
 Qed.
 
 Lemma refine_Join_Join_Filtered_Comp_Lists_filter_hd_andb
-: forall n heading1 heading2 headings
-         (f : ilist2 (n := n) (B := @RawTuple) headings -> bool)
-         (g : ilist2 (B := @RawTuple) (heading1 :: headings) -> bool)
-         (l2 : ilist2 (B := @RawTuple) headings -> Comp (list RawTuple))
-         (l2' : ilist2 (B := @RawTuple) (heading1 :: headings) -> Comp (list RawTuple))
-         (cond1 : ilist2 (B := @RawTuple) (heading1 :: headings) -> bool)
-         (cond2 : ilist2 (B := @RawTuple) (heading2 :: heading1 :: headings) -> bool),
+  : forall n heading1 heading2 headings
+           (f : ilist2 (n := n) (B := @RawTuple) headings -> bool)
+           (g : ilist2 (B := @RawTuple) (heading1 :: headings) -> bool)
+           (l2 : ilist2 (B := @RawTuple) headings -> Comp (list RawTuple))
+           (l2' : ilist2 (B := @RawTuple) (heading1 :: headings) -> Comp (list RawTuple))
+           (cond1 : ilist2 (B := @RawTuple) (heading1 :: headings) -> bool)
+           (cond2 : ilist2 (B := @RawTuple) (heading2 :: heading1 :: headings) -> bool),
     (forall a : ilist2 (B := @RawTuple) headings,
-     exists v : list RawTuple, refine (l2 a) (ret v)) ->
+        exists v : list RawTuple, refine (l2 a) (ret v)) ->
     forall l1 : list (ilist2 (B := @RawTuple) headings),
       refine
         (l <- Join_Filtered_Comp_Lists l1 l2 cond1;
@@ -697,34 +697,34 @@ Proof.
   - repeat setoid_rewrite refineEquiv_bind_unit; simpl; reflexivity.
   - case_eq (f a); simpl; intros a_eq v Comp_v.
     +  computes_to_inv; subst; computes_to_econstructor; eauto.
-      rewrite !filter_app, !filter_map, !map_app, !map_map in Comp_v'.
-      apply FlattenCompList.flatten_CompList_app_inv' in Comp_v'.
-      destruct_ex; split_and; subst.
-      assert (computes_to (l <- l <- FlattenCompList.flatten_CompList
-                             (map
-                                (fun l' : ilist2 (B := @RawTuple) headings =>
-                                   l <- l2 l';
-                                 ret (map (fun fa : RawTuple => icons2 fa l') l))
-                                (filter f l1));
-                           ret (filter cond1 l);
-                           l0 <- FlattenCompList.flatten_CompList
+       rewrite !filter_app, !filter_map, !map_app, !map_map in Comp_v'.
+       apply FlattenCompList.flatten_CompList_app_inv' in Comp_v'.
+       destruct_ex; split_and; subst.
+       assert (computes_to (l <- l <- FlattenCompList.flatten_CompList
                               (map
-                                 (fun l' : ilist2 (B := @RawTuple) (heading1 :: headings) =>
-                                    l0 <- l2' l';
-                                  ret (map (fun fa : RawTuple => icons2 fa l') l0))
-                                 (filter g l));
-                           ret (filter cond2 l0)) (filter cond2 x0)) as H'
-          by (repeat computes_to_econstructor; eauto).
-      pose (IHl1 l2 l2' cond1 cond2 H _ H');  computes_to_inv; subst.
-      computes_to_econstructor; eauto.
-      computes_to_econstructor.
-      repeat rewrite filter_app, filter_map.
-      repeat rewrite map_app, map_map; simpl.
-      rewrite filter_and, a_eq, filter_true.
-      eapply FlattenCompList.flatten_CompList_app; eauto.
-      rewrite !filter_app, <- c''; eauto.
+                                 (fun l' : ilist2 (B := @RawTuple) headings =>
+                                    l <- l2 l';
+                                  ret (map (fun fa : RawTuple => icons2 fa l') l))
+                                 (filter f l1));
+                            ret (filter cond1 l);
+                            l0 <- FlattenCompList.flatten_CompList
+                               (map
+                                  (fun l' : ilist2 (B := @RawTuple) (heading1 :: headings) =>
+                                     l0 <- l2' l';
+                                   ret (map (fun fa : RawTuple => icons2 fa l') l0))
+                                  (filter g l));
+                            ret (filter cond2 l0)) (filter cond2 x0)) as H'
+           by (repeat computes_to_econstructor; eauto).
+       pose (IHl1 l2 l2' cond1 cond2 H _ H');  computes_to_inv; subst.
+       computes_to_econstructor; eauto.
+       computes_to_econstructor.
+       repeat rewrite filter_app, filter_map.
+       repeat rewrite map_app, map_map; simpl.
+       rewrite filter_and, a_eq, filter_true.
+       eapply FlattenCompList.flatten_CompList_app; eauto.
+       rewrite !filter_app, <- c''; eauto.
     + destruct (H a); eauto.
-       computes_to_inv; subst; computes_to_econstructor; eauto.
+      computes_to_inv; subst; computes_to_econstructor; eauto.
       assert (computes_to (l <- l <- FlattenCompList.flatten_CompList
                              (map
                                 (fun l' : ilist2 (B := @RawTuple) headings =>
@@ -751,14 +751,14 @@ Qed.
 
 
 Lemma refine_Join_Join_Filtered_Comp_Lists_filter_hd
-: forall n heading1 heading2 headings
-         (f : ilist2 (n := n) (B := @RawTuple) headings -> bool)
-         (l2 : ilist2 (B := @RawTuple) headings -> Comp (list RawTuple))
-         (l2' : ilist2 (B := @RawTuple) (heading1 :: headings) -> Comp (list RawTuple))
-         (cond1 : ilist2 (B := @RawTuple) (heading1 :: headings) -> bool)
-         (cond2 : ilist2 (B := @RawTuple) (heading2 :: heading1 :: headings) -> bool),
+  : forall n heading1 heading2 headings
+           (f : ilist2 (n := n) (B := @RawTuple) headings -> bool)
+           (l2 : ilist2 (B := @RawTuple) headings -> Comp (list RawTuple))
+           (l2' : ilist2 (B := @RawTuple) (heading1 :: headings) -> Comp (list RawTuple))
+           (cond1 : ilist2 (B := @RawTuple) (heading1 :: headings) -> bool)
+           (cond2 : ilist2 (B := @RawTuple) (heading2 :: heading1 :: headings) -> bool),
     (forall a : ilist2 (B := @RawTuple) headings,
-     exists v : list RawTuple, refine (l2 a) (ret v)) ->
+        exists v : list RawTuple, refine (l2 a) (ret v)) ->
     forall l1 : list (ilist2 (B := @RawTuple) headings),
       refine
         (l <- Join_Filtered_Comp_Lists l1 l2 cond1;
@@ -771,7 +771,7 @@ Proof.
   setoid_rewrite filter_true in r.
   intros v Comp_v.
   apply r in Comp_v.
-   computes_to_inv; subst.
+  computes_to_inv; subst.
   rewrite filter_and, filter_true in Comp_v'.
   eauto.
 Qed.
@@ -783,8 +783,8 @@ Lemma List_Query_In_Return
       headings
       (l : list (ilist2 (n := n) (B := @RawTuple) headings))
       (r : ilist2 (B := @RawTuple) headings -> ResultT)
-: refine (List_Query_In l (fun tup => (Return (r tup))%QuerySpec))
-         (ret (map r l)).
+  : refine (List_Query_In l (fun tup => (Return (r tup))%QuerySpec))
+           (ret (map r l)).
 Proof.
   unfold List_Query_In; induction l; simpl; eauto.
   - reflexivity.
@@ -823,6 +823,155 @@ Proof.
   apply H; auto.
 Qed. *)
 
+
+Lemma refine_In_Where_Intersection heading
+  : forall R P (P_dec : DecideableEnsemble P),
+    refine
+      (QueryResultComp (Intersection (@IndexedRawTuple heading) R
+                                     (fun r => (P (indexedElement r)))) (fun r => Query_Return r))
+      (QueryResultComp R (fun r => Query_Where (P r)
+                                               (Query_Return r))).
+Proof.
+  unfold refine, In, QueryResultComp; intros * ? x H.
+  repeat computes_to_inv.
+  revert R x H H'.
+  induction v; simpl in *; intros; computes_to_inv; subst.
+  - repeat computes_to_econstructor.
+    instantiate (1 := @nil RawTuple); simpl.
+    inversion H; intuition; subst.
+    econstructor; split; eauto.
+    repeat split; intros; eauto.
+    eapply H0; inversion H2; subst; eauto.
+    eapply H0; eauto.
+    eapply in_map with (f := indexedElement) in H2; rewrite H1 in H2; destruct H2.
+    computes_to_econstructor.
+  - inversion H; destruct x; simpl in *; intuition;
+    try discriminate; injections.
+    assert (UnIndexedEnsembleListEquivalence
+              (fun t : IndexedRawTuple => elementIndex t <> elementIndex i
+                                          /\ R t) (map indexedElement x)).
+    { econstructor; intuition eauto.
+      inversion H1; subst.
+      apply H0 in H4; intuition.
+      subst; intuition eauto.
+      econstructor; intros; subst.
+      inversion H3; subst.
+      apply H6; eapply in_map_iff.
+      eexists; split; eauto.
+      eapply H0; eauto.
+      inversion H3; subst; eauto.
+    }
+    pose proof (IHv _ _ H1 H''); clear IHv; computes_to_inv.
+    inversion H'; subst.
+    refine pick val (List.app v0 v).
+    econstructor; intuition; eauto.
+    rewrite map_app; eapply FlattenCompList.flatten_CompList_app; eauto.
+    case_eq (dec (indexedElement i)); intros.
+    apply dec_decides_P in H6; apply H4 in H6; inversion H6; subst.
+    repeat computes_to_econstructor.
+    eapply Decides_false in H6; apply H5 in H6; subst; simpl;
+    computes_to_econstructor.
+    inversion H2; subst; intuition.
+    case_eq (dec (indexedElement i)); intros.
+    + apply dec_decides_P in H8; pose proof (H4 H8) as H'''; inversion H'''; subst.
+      econstructor 1.
+      instantiate (1 := List.app [i] x0); simpl; intuition eauto.
+      inversion H4; subst; apply H0 in H10; intuition.
+      right; eapply H6; econstructor; unfold In; eauto.
+      split; eauto; intros; subst.
+      inversion H3; subst; intuition eauto.
+      apply H15; eapply in_map_iff.
+      eexists; eauto.
+      eapply H0; eauto.
+      subst.
+      econstructor.
+      eapply H0; eauto.
+      unfold In; eauto.
+      econstructor; unfold In in *; eauto.
+      eapply H0; eauto.
+      rewrite <- H6 in H10; inversion H10; subst; unfold In in *; intuition.
+      eapply H0 in H13; eauto.
+      rewrite <- H6 in H10; inversion H10; subst; unfold In in *; intuition.
+      inversion H3; subst; econstructor; eauto.
+      intro; rewrite in_map_iff in H4; destruct_ex; intuition eauto.
+      apply H11; rewrite in_map_iff; destruct_ex; intuition eauto.
+      eexists; intuition eauto.
+      eapply H6 in H13; inversion H13; subst.
+      unfold In in H13.
+      inversion H13; subst.
+      inversion H15; subst; intuition.
+    + eapply Decides_false in H8; pose proof (H5 H8); subst; simpl.
+      inversion H2; subst; intuition.
+      econstructor 1.
+      instantiate (1 := x1); intuition eauto.
+      eapply H7.
+      repeat econstructor; eauto.
+      destruct H5; subst.
+      apply H0 in H5; intuition.
+      subst; intuition.
+      inversion H3; subst.
+      apply H17; apply in_map_iff; eexists; eauto.
+      destruct H5; eauto.
+      destruct H5; eauto.
+      eapply H7 in H5; destruct H5; destruct H5.
+      econstructor; eauto.
+Qed.
+
+Lemma refine_Where_Intersection heading {ResultT}
+  : forall R P (P_dec : DecideableEnsemble P) (bod : _ -> Comp (list ResultT)),
+    FiniteEnsemble R
+    -> refine
+         (QueryResultComp (heading := heading) R (fun r => Query_Where (P r) (bod r)))
+         (QueryResultComp (IndexedEnsemble_Intersection R P) bod)
+.
+Proof.
+  unfold refine, In, QueryResultComp; intros * ? ? Fin_R v Comp_v.
+  repeat computes_to_inv.
+  destruct Fin_R as [? Fin_R].
+  pose proof (UnIndexedEnsembleListEquivalence_filter P_dec Fin_R).
+  pose proof (Permutation_UnIndexedEnsembleListEquivalence' H Comp_v).
+  eapply PermutationFacts.permutation_filter in H0; destruct_ex;
+  intuition subst.
+  refine pick val x0; eauto using Permutation_UnIndexedEnsembleListEquivalence.
+  repeat computes_to_econstructor; eauto.
+  revert v Comp_v'; clear; induction x0; simpl; intros; eauto.
+  case_eq (dec a); simpl in *; intro H; rewrite H in *;
+  simpl in Comp_v'; computes_to_inv.
+  - computes_to_inv; subst; repeat computes_to_econstructor.
+    apply dec_decides_P in H; split; intros; intuition.
+    eapply IHx0; eauto.
+  - computes_to_inv; subst; repeat computes_to_econstructor.
+    apply Decides_false in H; split; intros; intuition.
+    eauto.
+    simpl; computes_to_econstructor.
+Qed.
+
+Lemma refine_Where_Intersection' heading {ResultT}
+  : forall R P (P_dec : P \/ ~ P) (bod : _ -> Comp (list ResultT)),
+    FiniteEnsemble R
+    -> refine
+         (QueryResultComp (heading := heading) R (fun r => Query_Where P (bod r)))
+         (Query_Where P (QueryResultComp R bod))
+.
+Proof.
+  unfold refine, In, Query_Where, QueryResultComp; intros * ? ? Fin_R v Comp_v.
+  intuition; computes_to_inv; intuition.
+  - computes_to_inv; refine pick val _; eauto.
+    repeat computes_to_econstructor.
+    eapply refine_flatten_CompList_func; eauto.
+    intros * ? ? ?; computes_to_econstructor.
+    computes_to_inv; intuition.
+  - subst.
+    destruct Fin_R as [? Fin_R].
+    computes_to_econstructor; eauto.
+    eapply refine_flatten_CompList_func.
+    intros * ? ? ?; computes_to_econstructor ; intuition.
+    revert H1.
+    instantiate (1 := fun _ => ret nil); simpl; intros; computes_to_inv;
+    subst; eauto.
+    clear; induction x; simpl; repeat computes_to_econstructor; eauto.
+Qed.
+
 Lemma DropQSConstraintsQuery_In {A} :
   forall qs_schema qs R bod,
     refine (@Query_In A qs_schema qs R bod)
@@ -838,7 +987,7 @@ Lemma DropQSConstraintsQuery_In_UnderBinder {A B} :
     (fun b : B => @Query_In A qs_schema qs R (bod b)) =
     (fun b : B => UnConstrQuery_In (DropQSConstraints qs) R (bod b)).
 Proof.
-    intros; unfold Query_In, UnConstrQuery_In, GetRelation, GetUnConstrRelation,
+  intros; unfold Query_In, UnConstrQuery_In, GetRelation, GetUnConstrRelation,
           DropQSConstraints; rewrite <- ith_imap2.
   reflexivity.
 Qed.
@@ -991,7 +1140,7 @@ Add Parametric Morphism
     (As : Vector.t A n)
     (a : A)
     (l' : list (ilist2 (B := f) As))
-: (@Join_Comp_Lists _ A f As a l')
+  : (@Join_Comp_Lists _ A f As a l')
     with signature
     (pointwise_relation _ refine) ==> refine
       as refine_Join_Comp_Lists.
@@ -1018,7 +1167,7 @@ Proof.
   split; intros; eauto.
   apply dec_decides_P in H0; intuition.
   apply Decides_false in H0; intuition.
-   computes_to_inv; eauto.
+  computes_to_inv; eauto.
 Qed.
 
 Lemma refineEquiv_For_DropQSConstraints A qsSchema qs :
@@ -1046,7 +1195,7 @@ Global Instance IndexedDecideableEnsemble
        {heading}
        {P : Ensemble (@RawTuple heading)}
        {P_dec : DecideableEnsemble P}
-: DecideableEnsemble (fun x : IndexedRawTuple => P (indexedRawTuple x)) :=
+  : DecideableEnsemble (fun x : IndexedRawTuple => P (indexedRawTuple x)) :=
   {| dec itup := @dec _ _ P_dec (indexedRawTuple itup)|}.
 Proof.
   intuition; eapply dec_decides_P; simpl in *; eauto.
